---
layout: default
title: 和の公式集
---

$$
n^{13} = \frac{15202 n}{5} - 3640 n^{3} + \frac{3003 n^{5}}{5}   + \frac{13!}{6!6!}\Sigma^{6,6} = \frac{n}{5}( 15202 - 18200 n^{2} +  3003 n^{4}) + \frac{13!}{6!6!}\sum_{k=1}^{n-1} (n-k)^{6}k^{6}
$$

$$
n^{14} = \frac{15202 n^{2}}{5}  - 3640 n^{4} + \frac{3003 n^{6}}{5} + \frac{14!}{6!7!}\Sigma^{6,7} = \frac{n^2}{5}( 15202 - 18200 n^{2} +  3003 n^{4}) + \frac{14!}{6!7!}\sum_{k=1}^{n-1} (n-k)^{6}k^{7}
$$

$$
n^{15} = 60060 n - 76010 n^{3}  + 16380 n^{5} - 429 n^{7} + \frac{15!}{7!7!}\Sigma^{7,7} = n(60060 - 76010 n^{2}  + 16380 n^{4} - 429 n^{6}) + \frac{15!}{7!7!}\sum_{k=1}^{n-1} (n-k)^{7}k^{7}
$$

$$
n^{16} =  60060 n^2 - 76010 n^{4}  + 16380 n^{6} - 429 n^{8} + \frac{16!}{7!8!}\Sigma^{7,8} = n^2(60060 - 76010 n^{2}  + 16380 n^{4} - 429 n^{6}) + \frac{16!}{7!8!}\sum_{k=1}^{n-1} (n-k)^{7}k^{8}
$$

$$
n^{17} = 1551693 n  - 2042040 n^{3} + 516868 n^{5} - 26520 n^{7} + \frac{17!}{8!8!}\Sigma^{8,8} = n( 1551693 - 2042040 n^{2} + 516868 n^{4} - 26520 n^{6}) + \frac{17!}{8!8!}\sum_{k=1}^{n-1} (n-k)^{8}k^{8}
$$

$$
n^{18} = 1551693 n^2  - 2042040 n^{4} + 516868 n^{6} - 26520 n^{8}  + \frac{18!}{8!9!}\Sigma^{8,9} = n^2 (1551693   - 2042040 n^{2} + 516868 n^{4} - 26520 n^{6} ) + \frac{18!}{8!9!}\sum_{k=1}^{n-1} (n-k)^{8}k^{9}
$$

$$
n^{19} =  \frac{1066406770 n}{21}  - 68791723 n^{3} + 19399380 n^{5} - \frac{9820492 n^{7}}{7}  + \frac{41990 n^{9}}{3} + \frac{19!}{9!9!}\Sigma^{9,9} = \frac{n}{21}(1066406770  - 1444626183 n^{2} + 407386980 n^{4} - 29461476 n^{6}  + 293930 n^{8}) + \frac{19!}{9!9!}\sum_{k=1}^{n-1} (n-k)^{9}k^{9}
$$

$$
n^{20} = \frac{1066406770 n^2}{21}  - 68791723 n^{4} + 19399380 n^{6} - \frac{9820492 n^{8}}{7}  + \frac{41990 n^{10}}{3} + \frac{20!}{9!10!}\Sigma^{9,10} = \frac{n^2}{21}(1066406770  - 1444626183 n^{2} + 407386980 n^{4} - 29461476 n^{6}  + 293930 n^{8}) + \frac{20!}{9!10!}\sum_{k=1}^{n-1} (n-k)^{9}k^{10}
$$
